RegexCorrectness/VM/CharStep/Lemmas.lean
@@ -13,19 +13,20 @@ open String (Pos Iterator)
 namespace Regex.VM
 
 variable {nfa : NFA} {wf : nfa.WellFormed} {it : Iterator}
-  {current next : SparseSet nfa.nodes.size} {updates : Vec (List (Nat × String.Pos)) nfa.nodes.size}
+  {current : SearchState' nfa} {currentUpdates : Vec (List (Nat × Pos)) nfa.nodes.size}
+  {next : SparseSet nfa.nodes.size} {updates : Vec (List (Nat × String.Pos)) nfa.nodes.size}
   {state : Fin nfa.nodes.size}
   {next' : SparseSet nfa.nodes.size} {matched' : Option (List (Nat × Pos))}
   {updates' : Vec (List (Nat × String.Pos)) nfa.nodes.size}
 
-theorem stepChar.lower_bound (h : stepChar' nfa wf it next updates state = (next', matched', updates'))
+theorem stepChar.lower_bound (h : stepChar' nfa wf it currentUpdates next updates state = (next', matched', updates'))
   (lb : εClosure.LowerBound next) :
   εClosure.LowerBound next' := by
   simp [stepChar'] at h
   split at h
   next c' state' hn =>
     split at h
-    next eq => exact εClosure.lower_bound h lb
+    next => exact εClosure.lower_bound h lb
     next => simp_all
   next cs state' =>
     split at h
@@ -33,8 +34,23 @@ theorem stepChar.lower_bound (h : stepChar' nfa wf it next updates state = (next
     next => simp_all
   next => simp_all
 
+theorem stepChar.eq_updates_of_mem_next {i k} (h : stepChar' nfa wf it currentUpdates next updates i = (next', matched', updates'))
+  (mem : k ∈ next) :
+  updates'[k] = updates[k] := by
+  simp [stepChar'] at h
+  split at h
+  next c' j hn =>
+    split at h
+    next eq => exact εClosure.eq_updates_of_mem_next h mem
+    next => simp_all
+  next cs j =>
+    split at h
+    next => exact εClosure.eq_updates_of_mem_next h mem
+    next => simp_all
+  next => simp_all
+
 theorem mem_next_of_stepChar {l m r i j k update}
-  (h : stepChar' nfa wf it next updates i = (next', matched', updates'))
+  (h : stepChar' nfa wf it currentUpdates next updates i = (next', matched', updates'))
   (lb : εClosure.LowerBound next)
   (step : nfa.CharStep l m it.curr r i j) (cls : nfa.εClosure' ⟨l, it.curr :: m, r⟩ j k update) :
   k ∈ next' := by
@@ -53,13 +69,13 @@ theorem mem_next_of_stepChar {l m r i j k update}
     simp_all
 
 theorem write_updates_of_mem_next_of_stepChar {i k} (span : Span) (hspan : span.iterator = it)
-  (h : stepChar' nfa wf it next updates i = (next', matched', updates'))
+  (h : stepChar' nfa wf it currentUpdates next updates i = (next', matched', updates'))
   (notEnd : ¬it.atEnd) (mem : k ∈ next') :
   k ∈ next ∨ ∃ r' j update',
     span.r = it.curr :: r' ∧
     nfa.CharStep span.l span.m it.curr r' i j ∧
     nfa.εClosure' span.next j k update' ∧
-    (WriteUpdate k → updates'[k] = updates.get i i.isLt ++ update') := by
+    (WriteUpdate k → updates'[k] = currentUpdates.get i i.isLt ++ update') := by
   simp [stepChar'] at h
   split at h
   next c j hn =>
@@ -101,38 +117,61 @@ theorem eachStepChar.go.lower_bound {i hle} (h : eachStepChar'.go nfa wf it curr
     rw [eachStepChar'.go_not_found hlt h' not_found] at h
     exact ih h (stepChar.lower_bound h' lb)
 
-def eachStepChar.Inv (nfa : NFA) (wf : nfa.WellFormed) (it : Iterator) (next : SparseSet nfa.nodes.size) (updates : Vec (List (Nat × Pos)) nfa.nodes.size) : Prop :=
+def eachStepChar.Inv (nfa : NFA) (wf : nfa.WellFormed) (it : Iterator)
+  (next : SparseSet nfa.nodes.size) (updates : Vec (List (Nat × Pos)) nfa.nodes.size) : Prop :=
   ∀ i ∈ next, ∃ span update, span.iterator = it ∧ nfa.VMPath wf span i update ∧ (WriteUpdate i → updates[i] = update)
+
+theorem eachStepChar.Inv.of_empty (h : next.isEmpty) : eachStepChar.Inv nfa wf it next updates := by
+  intro i mem
+  exact (SparseSet.not_mem_of_isEmpty h mem).elim
+
+theorem eachStepChar.Inv.of_stepChar {idx} (hlt : idx < current.states.count)
+  (h : stepChar' nfa wf it current.updates next updates current.states[idx] = (next', matched', updates'))
+  (notEnd : ¬it.atEnd)
+  (inv_curr : eachStepChar.Inv nfa wf it current.states current.updates)
+  (inv_next : eachStepChar.Inv nfa wf it.next next updates) :
+  eachStepChar.Inv nfa wf it.next next' updates' := by
+  have ⟨span, update, eqit, path, write⟩ := inv_curr current.states[idx] (SparseSet.mem_get hlt)
+
+  intro k mem
+  have := write_updates_of_mem_next_of_stepChar span eqit h (by simp [notEnd]) mem
+  match this with
+  | .inl mem =>
+    have inv := inv_next k mem
+    have equ := stepChar.eq_updates_of_mem_next h mem
+    exact equ ▸ inv
+  | .inr ⟨r', j, update', eqr, step, cls, write'⟩ =>
+    simp [step.write_update] at write
+    have write'' : WriteUpdate k → updates'[k] = update ++ update' := write ▸ write'
+    exact ⟨span.next, update ++ update', by rw [Span.next_iterator eqr, eqit], .more path eqr step cls, write''⟩
 
 theorem eachStepChar.go.inv {idx hle} (h : eachStepChar'.go nfa wf it current idx hle next updates = (next', matched', updates'))
   (notEnd : ¬it.atEnd)
-  (inv_curr : eachStepChar.Inv nfa wf it current updates) (inv_next : eachStepChar.Inv nfa wf it.next next updates) :
+  (inv_curr : eachStepChar.Inv nfa wf it current.states current.updates)
+  (inv_next : eachStepChar.Inv nfa wf it.next next updates) :
   eachStepChar.Inv nfa wf it.next next' updates' := by
   induction idx, hle, next, updates using eachStepChar'.go.induct' nfa wf it current with
   | base next updates => simp_all
   | found idx next updates hlt next'' matched updates'' h' found =>
     rw [eachStepChar'.go_found hlt h' found] at h
     simp_all
-    have ⟨span, update, eqit, path, write⟩ := inv_curr current[idx] (SparseSet.mem_get hlt)
-
-    intro k mem
-    have := write_updates_of_mem_next_of_stepChar span eqit h' (by simp [notEnd]) mem
-    match this with
-    | .inl mem =>
-      -- missing `updates'[k] = updates[k]`
-      -- exact inv_next k mem
-      sorry
-    | .inr ⟨r', j, update', eqr, step, cls, write'⟩ =>
-      -- CharStep implies WriteUpdate
-      have : WriteUpdate current[idx] := sorry
-      simp [this] at write
-      have write'' : WriteUpdate k → updates'[k] = update ++ update' := write ▸ write'
-      refine ⟨span.next, update ++ update', by rw [Span.next_iterator eqr, eqit], .more path eqr step cls, write''⟩
+    exact eachStepChar.Inv.of_stepChar hlt h' (by simp [notEnd]) inv_curr inv_next
   | not_found idx next updates hlt next'' matched updates'' h' not_found ih =>
     rw [eachStepChar'.go_not_found hlt h' not_found] at h
-    -- FIXME: WE HAVE A BUG. We shouldn't share `updates` between `current` and `next` since the
-    -- writes for the previous indices can pollute the updates of the remaining indices while iterating
-    -- through `next`.
-    apply ih h sorry sorry
+    have inv' : eachStepChar.Inv nfa wf it.next next'' updates'' :=
+      eachStepChar.Inv.of_stepChar hlt h' (by simp [notEnd]) inv_curr inv_next
+    apply ih h inv'
+
+theorem eachStepChar.inv {next next'} (h : eachStepChar' nfa wf it current next = (next', matched'))
+  (notEnd : ¬it.atEnd) (empty : next.states.isEmpty)
+  (inv : eachStepChar.Inv nfa wf it current.states current.updates) :
+  eachStepChar.Inv nfa wf it.next next'.states next'.updates := by
+  simp [eachStepChar'] at h
+  set result := eachStepChar'.go nfa wf it current 0 (Nat.zero_le _) next.states next.updates
+  set nextStates := result.1
+  set nextUpdates := result.2.2
+  have : result = (nextStates, matched', nextUpdates) := by
+    simp [←h]
+  exact h.1 ▸ eachStepChar.go.inv this notEnd inv (eachStepChar.Inv.of_empty empty)
 
 end Regex.VM
